AllStar/ParserTests.v
@@ -1,0 +1,36 @@
+Require Import String List.
+Require Import AllStar.Parser ExampleGrammars
+               Grammar Subparser Lib.Utils.
+Import ListNotations.
+
+Print g311.
+(*
+[(NT "S", [T "if"; NT "E"; T "then"; NT "S"; T "else"; NT "S"]);
+ (NT "S", [T "begin"; NT "S"; NT "L"]);
+ (NT "S", [T "print"; NT "E"]); (NT "L", [T "end"]);
+ (NT "L", [T ";"; NT "S"; NT "L"]);
+ (NT "E", [T "num"; T "=="; T "num"])]
+*)
+
+Definition prog1 :=
+  tokenize "if num == num then print num == num else print num == num".
+
+Example test1 :
+    parse g311 (NT "S") prog1 100 = (Some g311ParseTree1, nil).
+Proof. reflexivity. Qed.
+
+Definition prog2 := tokenize "begin print num == num end".
+
+Example test2 :
+  exists tr suf,
+    parse g311 (NT "S") prog2 100 = (Some tr, suf).
+Proof. compute. repeat eexists. Qed.
+
+Definition prog3 :=
+  tokenize "begin print num == num ; print num == num end".
+
+Example test3 :
+  exists tr suf,
+    parse g311 (NT "S") prog3 100 = (Some tr, suf).
+Proof. compute. repeat eexists. Qed.
+           
